providers/evercrypt/EverCrypt.Hash.fsti
@@ -234,7 +234,8 @@ val alloca: a:alg -> StackInline (state a)
     M.(loc_includes (loc_region_only true (HS.get_tip h1)) (footprint s h1))))
 
 val create_in: a:alg -> r:HS.rid -> ST (state a)
-  (requires (fun _ -> HyperStack.ST.is_eternal_region r))
+  (requires (fun _ ->
+    HyperStack.ST.is_eternal_region r))
   (ensures (fun h0 s h1 ->
     invariant s h1 /\
     M.(modifies loc_none h0 h1) /\
